Explanation:
$$\sum_{i=0}^{to-1}\left\lfloor \frac{ki+c}{m}\right\rfloor=\sum_{x=1}^{to}\left\lfloor \frac{k(to-x)+c}{m}\right\rfloor$$
This is equal the number of lattice points $(x,y)$ such that $x,y>0$ and
$$y\le \left\lfloor \frac{k(to-x)+c}{m}\right\rfloor\implies my+kx\le k\cdot to+c.$$
If we swap $x,y$ then the sum is equal to
\begin{align*}
\sum_{y=1}^{to2}\left\lfloor \frac{k\cdot to+c-my}{k}\right\rfloor&=\sum_{y=1}^{to2}\left\lfloor \frac{k\cdot to+c-my}{k}\right\rfloor\\
&=\sum_{y=1}^{to2}to+\left\lfloor \frac{c-my}{k}\right\rfloor\\
&=to\cdot to2-\sum_{y=1}^{to2}\left\lceil \frac{my-c}{k}\right\rceil\\
&=to\cdot to2-\sum_{y=1}^{to2}\left\lfloor \frac{my-c+k-1}{k}\right\rfloor\\
&=to\cdot to2-\sum_{y=0}^{to2-1}\left\lfloor \frac{my+m-c+k-1}{k}\right\rfloor\\
&=(to-1)\cdot to2-\sum_{y=0}^{to2-1}\left\lfloor \frac{my+m-c-1}{k}\right\rfloor
\end{align*}
as desired.